Move Int Instance to prelude

theories/lib/prelude.v
@@ -1,7 +1,7 @@
 (* Re-export of Iris and some general stuff *)
 
 From iris_os.lib Require Export CpdtTactics Integers.
-Require Import iris.prelude.prelude.
+From iris.prelude Require Import prelude countable.
 Open Scope Z_scope.
 
 Definition ident : Set := Z.
@@ -43,3 +43,20 @@ Proof.
   - simpl. intros. inversion H.
     apply Finj in H1. apply IHl1 in H2. by subst.
 Qed.
+
+Global Instance int32_eq_dec: EqDecision int32 := Int.eq_dec.
+
+Definition int32_encode (i: int32) : positive := encode (Int.unsigned i).
+Definition int32_decode (p: positive) : option int32 :=
+  match decode p with
+    | Some z => Some (Int.repr z)
+    | None => None
+  end.
+
+Lemma int32_decode_encode i: int32_decode (int32_encode i) = Some i.
+Proof. unfold int32_encode, int32_decode. rewrite decode_encode.
+       f_equal. apply Int.repr_unsigned.
+Qed.
+
+Global Instance int32_countable: Countable int32 :=
+  Build_Countable _ _ int32_encode int32_decode int32_decode_encode.
