theories/os/page_table.v
@@ -2,9 +2,6 @@
 
 Require Import iris_os.clang.logic.
 
-Instance int32_eq_dec: EqDecision int32 := Int.eq_dec.
-Instance int32_countable: Countable int32. Admitted.
-
 Definition option_addr_to_val (opt_a: option addr) : val :=
   match opt_a with
     | Some a => Vptr a
